lot of implementations

Graphs/Graph.lean
@@ -6,15 +6,26 @@ namespace GraphTheory
 abbrev Node := Nat
 
 @[simp]
-def unique [BEq a] (as : List a) := (as ≠ []) → ∀ a ∈ as, (as.filter (. == a)).length = 1
+def unique [BEq a] (as : List a) : Prop :=
+match as with
+| [] => true
+| a::as => if List.filter (fun x => x == a) as == [] then unique as else false
 
-instance  [BEq a] {as : List a} : Decidable  (unique as) := by
-  rw [unique]
+def uniqueB [BEq a] (as : List a) : Bool :=
+match as with
+| [] => true
+| a::as => if List.filter (fun x => x == a) as == [] then uniqueB as else false
+
+theorem unique_uniqueB_iff [BEq a] {as : List a}: uniqueB as ↔ unique as := by
   induction as with
-  | nil => simp; exact instDecidableTrue
+  | nil => rfl
   | cons a as ih =>
+    rw [unique, uniqueB]
     simp
-    exact instDecidableAnd
+    exact fun _ => ih
+
+instance  [BEq a] {as : List a} : Decidable  (unique as) :=
+  decidable_of_bool _ unique_uniqueB_iff
 
 -- Edge ---------------------------------
 
@@ -91,6 +102,8 @@ def K0 := instInhabitedGraph.default
 #eval K2
 #eval K3
 
+
+
 #eval K1.isTrivial
 #eval K2.isTrivial
 #eval K3.isTrivial
@@ -99,12 +112,12 @@ def K0 := instInhabitedGraph.default
 
 #eval K 7 (by simp; decide)
 
+#eval (K 4 (by simp; decide)).adjacent 1 1
+
 def e1 := (K3.E.get? 1).get (by decide)
 def e2 := (K3.E.get? 2).get (by decide)
 
 #eval Graph.parallel K3 e1 e2
-
-
 
 def L (n : Node) (l : List (Node × (Node × Int))) : Int :=
 match l.filter (λ (x,_) => x == n) with
@@ -122,9 +135,10 @@ match l with
 | x::xs => if n == x.1 then (n,(x.2.1, v))::xs else x::(newL n v xs)
 
 #eval newL 2 4 [(2,(0,1)), (3,(0,1))]
-#eval L 2  <| newL 2 4 [(2,(0,1)), (3,(0,1))]
-#eval LPair 2 [(2, 0, 4), (3, 0, 1)]
+#eval L 2  [(2,(0,4)), (3,(0,1))]
+#eval LPair 2 [(2, (0, 4)), (3, (0, 1))]
 
+-- Weighted graphs
 structure WGraph where
   N : List Node
   E : List Edge
@@ -146,7 +160,6 @@ instance : Repr WGraph where
 
 #eval WGraph.mk [1,2,3] [Edge.mk 1 1 2, Edge.mk 2 2 3] [((Edge.mk 1 1 2), 3), ((Edge.mk 2 2 3), 1)] (by simp)
 
-
 def findMinL  (v : (Node × Int)) (l : List (Node × (Node × Int))) : (Node × Int) :=
 match l with
 | [] => v
@@ -160,10 +173,10 @@ def MinLNode (p : Node × (Node × Int)) (l : List (Node × (Node × Int))) : No
 
 #eval (fun x => MinLNode (0,x) [(1,0,3), (2,0,2), (3,0,1), (4,0,3)]) <| findMinL (0,-1) [(1,0,2), (2,0,2), (3,0,1), (4,0,3)]
 
-def new_Ls (ns : List Node) (v : Int) : List (Node × (Node × Int)) :=
+def newLs (ns : List Node) (v : Int) : List (Node × (Node × Int)) :=
 ns.map (fun x => (x,(0, v)))
 
-#eval newL 1 0 <| new_Ls (K 3 (by simp; decide)).N (-1)
+#eval newLs (K 3 (by simp; decide)).N (-1)
 
 def Node.adjacent (es : List Edge) (n m : Node) := ∃ e, e ∈ es ∧ e.incident n ∧ e.incident m ∧ n ≠ m
 
@@ -175,7 +188,6 @@ def filterAdj (n : Node) (g : List Node) (es : List Edge) : List Node :=
   g.filter (Node.adjacent es n)
 
 #eval filterAdj 1 (K 4 (by simp; decide)).N (K 4 (by simp; decide)).E
-#eval (K 4 (by simp; decide)).adjacent 1 1
 
 def findWeight (v n : Node) (ws : List (Edge × Int)) : Int :=
   match ws with
@@ -197,25 +209,25 @@ def updateLs (v n : Node) (l : List (Node × (Node × Int))) (ws : List (Edge ×
     | [] => []
     | x::xs => if x.1 == n then (n,(v,label))::xs else x::(help n xs label)
 
-def UpdateLsMap (v : Node) (ns : List Node) (l : List (Node × (Node × Int)))  (ws : List (Edge × Int))
+def updateLsMap (v : Node) (ns : List Node) (l : List (Node × (Node × Int)))  (ws : List (Edge × Int))
   : List (Node × (Node × Int)) :=
   List.foldr (fun x y => updateLs v x y ws) l ns
 
-#eval UpdateLsMap 1 [2, 3] [(1, 0, 2), (2, 0, 4), (3, 0, 4)] [(Edge.mk 1 1 3, 1), (Edge.mk 1 1 2, 1)]
-#eval UpdateLsMap 1 [2, 3] [(1, 0, 2), (2, 0, 4), (3, 0, 4)] [(Edge.mk 1 1 3, 3), (Edge.mk 1 1 2, 4)]
+#eval updateLsMap 1 [2, 3] [(1, 0, 2), (2, 0, 4), (3, 0, 4)] [(Edge.mk 1 1 3, 1), (Edge.mk 1 1 2, 1)]
+#eval updateLsMap 1 [2, 3] [(1, 0, 2), (2, 0, 4), (3, 0, 4)] [(Edge.mk 1 1 3, 3), (Edge.mk 1 1 2, 4)]
 
 def isinGraph (n : Node) (ns : List Node) : Bool :=
   if (ns.filter (· == n)).length >= 1 then true else false
 
 #eval isinGraph 1 [2,3]
 
-def t1 : (new_Ls [a] (-1))++(new_Ls as (-1)) = new_Ls (a::as) (-1) := by
+def t1 : (newLs [a] (-1))++(newLs as (-1)) = newLs (a::as) (-1) := by
       induction as with
       | nil => rfl
       | cons b bs _ =>
         rfl
 
-example : ∀ v, v ∈ T → (fun x => MinLNode (0,x) (UpdateLsMap v (filterAdj v T es) (new_Ls T (-1)) ws)) (findMinL (0,-1)  (UpdateLsMap v (filterAdj v T es) (new_Ls T (-1)) ws)) ∈ T := by
+example : ∀ v, v ∈ T → (fun x => MinLNode (0,x) (updateLsMap v (filterAdj v T es) (newLs T (-1)) ws)) (findMinL (0,-1)  (updateLsMap v (filterAdj v T es) (newLs T (-1)) ws)) ∈ T := by
   simp
   induction T with
   | nil => simp
@@ -226,9 +238,9 @@ example : ∀ v, v ∈ T → (fun x => MinLNode (0,x) (UpdateLsMap v (filterAdj 
     simp
     sorry
 
--- definition still partial
+-- partial definition
 partial def dijkstra (a z : Node) (G : Graph) (W : List (Edge × Int)) : List (Node × (Node × Int)) :=
-  let labels := newL a 0 <|new_Ls G.N (-1)
+  let labels := newL a 0 <|newLs G.N (-1)
   let T := G.N
   if T.length = 0 then [(0,(0,0))] else
     help  z T labels T G.E W [] where
@@ -239,7 +251,7 @@ partial def dijkstra (a z : Node) (G : Graph) (W : List (Edge × Int)) : List (N
         let v := (fun x => MinLNode (0,x) ls) <| findMinL (0,-1) ls
         let v_l := (LPair v ls)
         let ads := filterAdj v N es
-        let new_lbs := List.filter (fun x => x.1 != v) (UpdateLsMap v ads ls ws)
+        let new_lbs := List.filter (fun x => x.1 != v) (updateLsMap v ads ls ws)
         let T := t.filter (fun x => x != v)
         help z T new_lbs N es ws (f++[v_l])
       else f
@@ -257,13 +269,13 @@ match W with
 #eval ChangeW 3 (Edge.mk 1 1 2) <| SimpleW (K 4 (by simp; decide)).E
 #eval dijkstra 1 3 (K 3 (by simp; decide)) [(Edge.mk 1 1 3, 5), (Edge.mk 2 1 2, 1), (Edge.mk 3 3 2, 1)]
 
-
--- hamiltonian paths
+-- walks, paths and cycles
 def casB (m n : Node) (E : List Edge) : Bool :=
 match E with
 | [] => if m == n then true else false
 | a::as => if m == a.i then casB a.j n as else false
 
+-- the cas function is inspired in the Isabelle's definition of walk, path and cycle
 def cas (m n : Node) (E : List Edge) : Prop :=
 match E with
 | [] => if m == n then true else false
@@ -278,36 +290,120 @@ theorem cas_casB_iff : casB m n E ↔ cas m n E := by
 instance : Decidable (cas m n E) := decidable_of_bool _ cas_casB_iff
 
 #eval cas 1 3 [Edge.mk 1 1 2, Edge.mk 2 2 3]
+#eval cas 1 2 [Edge.mk 1 1 2, Edge.mk 2 2 3]
 
-def FirstNode (E : List Edge) : Node :=
+def firstNode (E : List Edge) : Node :=
   match E with
   | [] => 0
   | a::_ => a.i
 
-def LastNode (n : Node) (E : List Edge) : Node :=
+def lastNode (n : Node) (E : List Edge) : Node :=
   match E with
   | [] => n
-  | a::as => LastNode a.j as
+  | a::as => lastNode a.j as
 
 structure Walk where
   start : Node
-  walk : List Edge
-  ok : cas start (LastNode start walk) walk
-       ∧ ((walk = []) ∨ start = (FirstNode walk))
+  aWalk : List Edge
+  ok : cas start (lastNode start aWalk) aWalk
+       ∧ ((aWalk = []) ∨ start = (firstNode aWalk))
 
 instance : Repr Walk where
   reprPrec w _ :=
     let formatEdge := fun n => (f!"v{n.i}~v{n.j}")
     let formatNode := fun n => (f!"v{n}")
-    f!"{[formatNode w.start]++(List.map formatEdge w.walk)++[formatNode (LastNode w.start w.walk)]}"
+    f!"{[formatNode w.start]++(List.map formatEdge w.aWalk)++[formatNode (lastNode w.start w.aWalk)]}"
 
 #eval Walk.mk 1 [Edge.mk 1 1 2, Edge.mk 2 2 1] (by simp; exact ite_some_none_eq_some.mp rfl)
 #eval cas 1 0 [Edge.mk 1 1 2, Edge.mk 2 6 0]
 
+#eval (K 2 (by simp;decide)).N ++ (K 3 (by simp; decide)).N
+
+def Walk.nodes (w : Walk) : List Node :=
+  [w.start] ++ help w.aWalk where
+  help (walk : List Edge) : List Node :=
+    match walk with
+    | [] => []
+    | a::as => [a.j]++(help as)
+
+#eval (Walk.mk 1 [Edge.mk 1 1 2, Edge.mk 2 2 3] (by simp; exact ite_some_none_eq_some.mp rfl)).nodes
+
+def isSimple (w : Walk) : Prop :=
+  if unique (w.nodes) then true else false
+
+instance : Decidable (isSimple w) := by
+  rw [isSimple]
+  exact (if unique w.nodes then true else false).decEq true
+
 structure Path where
-  path : Walk
-  -- isSimple := isSimple path
-  ok : unique path.walk
+  aWalk : Walk
+  isSimple := isSimple aWalk
+  ok : unique aWalk.aWalk
+-- deriving Repr
+
+instance : Repr Path where
+  reprPrec w _ :=
+    let formatEdge := fun n => (f!"v{n.i}~v{n.j}")
+    let formatNode := fun n => (f!"v{n}")
+    f!"{[formatNode w.aWalk.start]++(List.map formatEdge w.aWalk.aWalk)++[formatNode (lastNode w.aWalk.start w.aWalk.aWalk)]}"
+
+def wlk := (Walk.mk 1 [Edge.mk 1 1 2, Edge.mk 2 2 3] (by simp; exact ite_some_none_eq_some.mp rfl))
+#eval (Path.mk wlk (isSimple wlk) (by simp)).isSimple
+#eval (Path.mk wlk (isSimple wlk) (by simp))
+def owlk := (Walk.mk 1 [Edge.mk 1 1 2, Edge.mk 1 2 1] (by simp; exact ite_some_none_eq_some.mp rfl))
+#eval (Path.mk owlk (isSimple owlk) (by simp))
+
+structure Cycle where
+  aWalk : Walk
+  ok : aWalk.start = (lastNode aWalk.start aWalk.aWalk)
+     ∧ unique aWalk.aWalk
+
+instance : Repr Cycle where
+  reprPrec w _ :=
+    let formatEdge := fun n => (f!"v{n.i}~v{n.j}")
+    let formatNode := fun n => (f!"v{n}")
+    f!"{[formatNode w.aWalk.start]++(List.map formatEdge w.aWalk.aWalk)++[formatNode (lastNode w.aWalk.start w.aWalk.aWalk)]}"
+
+#eval Cycle.mk (Walk.mk 1 [Edge.mk 1 1 2, Edge.mk 2 2 1] (by simp; exact ite_some_none_eq_some.mp rfl)) (by simp; rw [lastNode, lastNode, lastNode])
+#eval (Cycle.mk (Walk.mk 1 [Edge.mk 1 1 2, Edge.mk 2 2 1] (by simp; exact ite_some_none_eq_some.mp rfl)) (by simp; rw [lastNode, lastNode, lastNode])).aWalk.nodes
+
+-- Euler graphs
+
+structure EulerPath where
+  G : Graph
+  aPath : Path
+  ok : ∀e, e ∈ G.E → e ∈ aPath.aWalk.aWalk
+     ∧ ∀n, n ∈ G.N → n ∈ aPath.aWalk.nodes
+
+instance : Repr EulerPath where
+  reprPrec w _ :=
+    let formatEdge := fun n => (f!"v{n.i}~v{n.j}")
+    let formatNode := fun n => (f!"v{n}")
+    f!"{[formatNode w.aPath.aWalk.start]++(List.map formatEdge w.aPath.aWalk.aWalk)++[formatNode (lastNode w.aPath.aWalk.start w.aPath.aWalk.aWalk)]}"
+
+
+def G1 := Graph.mk [1,2,3] [Edge.mk 1 1 2, Edge.mk 2 2 3] (by simp)
+#eval EulerPath.mk G1 (Path.mk (Walk.mk 1  [Edge.mk 1 1 2, Edge.mk 2 2 3] (by simp; decide)) (isSimple (Walk.mk 1  [Edge.mk 1 1 2, Edge.mk 2 2 3] (by simp; decide))) (by exact rfl)) (by simp; decide)
+
+
+-- the Isabelle's graphs paper implementation doesn't require that the cycle to contain every node
+-- of the graph G.
+-- but, as in our classes we've stated that it needs to contain all the nodes, the implementation
+-- below also has that requirement.
+structure EulerCycle where
+  G : Graph
+  aCycle : Cycle
+  ok : ∀e, e ∈ G.E → e ∈ aCycle.aWalk.aWalk
+     ∧ ∀n, n ∈ G.N → n ∈ aCycle.aWalk.nodes
+
+instance : Repr EulerCycle where
+  reprPrec w _ :=
+    let formatEdge := fun n => (f!"v{n.i}~v{n.j}")
+    let formatNode := fun n => (f!"v{n}")
+    f!"{[formatNode w.aCycle.aWalk.start]++(List.map formatEdge w.aCycle.aWalk.aWalk)++[formatNode (lastNode w.aCycle.aWalk.start w.aCycle.aWalk.aWalk)]}"
+
+
+#eval EulerCycle.mk K3 (Cycle.mk (Walk.mk 1 [Edge.mk 1 1 2, Edge.mk 2 2 3, Edge.mk 3 3 1] (by simp; exact ite_some_none_eq_some.mp rfl)) (by simp; decide)) (by simp; decide)
 
 
 def Degree (n : Node) (E : List Edge) : Nat :=
@@ -316,9 +412,85 @@ match E with
 | x::xs => if x.i == n ∨ x.j == n then 1 + (Degree n xs) else Degree n xs
 
 #eval Degree 1 (K 4 (by simp; decide)).E
-#eval [1,2,3].filter (fun x => ) [1,2,3,4,5]
+
+def hasECycle (G : Graph) : Prop :=
+  ∀ n ∈ G.N, (Degree n G.E) % 2 = 0
+
+instance : Decidable (hasECycle G) := by
+  simp [hasECycle]
+  exact List.decidableBAll (fun x => Degree x G.E % 2 = 0) G.N
+
+#eval hasECycle K3
+#eval hasECycle (K 4 (by simp;decide))
 
 
+def ECyclePair (G : Graph) : Prop :=
+  ∃ (EC : EulerCycle), EC.G = G
+
+-- the theorem can't be proven because it needs another inductive
+theorem EulerCycle_iff (G : Graph) :  (∀ n ∈ G.N, Degree n G.E % 2 = 0) ↔ ∃ (EC : EulerCycle), EC.G = G := by
+  induction G.E with
+  |nil =>  sorry
+  |cons a as ih => sorry
+
+theorem Pair_ECycle_iff (G : Graph) : hasECycle G ↔ ECyclePair G := by rw [hasECycle, ECyclePair]; apply EulerCycle_iff
+
+instance : Decidable (ECyclePair G) := decidable_of_iff (_) (by apply EulerCycle_iff)
+
+-- Hamiltonian Graphs
+
+structure HamCycle where
+  G : Graph
+  aCycle : Cycle
+  ok : ∀ n ∈ G.N, n ∈ aCycle.aWalk.nodes
+     ∧ unique (aCycle.aWalk.nodes.filter (λ x => x != aCycle.aWalk.start))
+
+instance : Repr HamCycle where
+  reprPrec w _ :=
+    let formatEdge := fun n => (f!"v{n.i}~v{n.j}")
+    let formatNode := fun n => (f!"v{n}")
+    f!"{[formatNode w.aCycle.aWalk.start]++(List.map formatEdge w.aCycle.aWalk.aWalk)++[formatNode (lastNode w.aCycle.aWalk.start w.aCycle.aWalk.aWalk)]}"
+
+
+#eval HamCycle.mk K3 (Cycle.mk (Walk.mk 1 [Edge.mk 1 1 2, Edge.mk 2 2 3, Edge.mk 3 3 1] (by simp; decide)) (by simp; decide)) (by simp; decide)
+
+-- first try of implementing a sufficient condition checker
+def old_hasHamCycle (G : Graph) : Prop :=
+  ∀m n, m ∈ G.N ∧ n ∈ G.N ∧ ¬(G.adjacent m n) -> Degree m G.E + Degree n G.E ≥ G.N.length
+
+def hasHam (G:Graph) (N:List Node) : Prop :=
+  match N with
+  | [] => true
+  | t::ts =>
+    let D := G.N.length
+    if ∀n ∈ ts, Degree n G.E + Degree t G.E ≥ D then hasHam G ts else false
+
+def hasHamB (G:Graph) (N:List Node) : Bool :=
+  match N with
+  | [] => true
+  | t::ts =>
+    let D := G.N.length
+    if ∀n ∈ ts, Degree n G.E + Degree t G.E ≥ D then hasHamB G ts else false
+
+def hasHam_hasHamB_iff {G : Graph} {N : List Node} : hasHamB G N  ↔ hasHam G N:= by
+  induction N with
+  | nil =>
+    rfl
+  | cons t ts ih =>
+    simp [hasHam, hasHamB]
+    exact fun _ => ih
+
+instance : Decidable (hasHam G N) := decidable_of_bool _ hasHam_hasHamB_iff
+
+abbrev hasHamCycle (G : Graph) : Prop := hasHam G G.N
+
+#eval hasHamB K3 K3.N
+#eval hasHam K3 K3.N
+#eval hasHamCycle K3
+
+-- this decidable is not provable with what we currently have
+def isConnected (G : Graph) : Prop :=
+  ∀ m n, m ∈ G.N ∧ n ∈ G.N → ∃ (P : Path), P.aWalk.start = m ∧ lastNode P.aWalk.start P.aWalk.aWalk = n
 
 -- isomorphism
 @[simp]
@@ -353,48 +525,79 @@ structure oGraph where
   ok : ∀ e ∈ E, (t e) ∈ N ∧ (h e) ∈ N
 
 
-
+#eval isSubGraph (K 3 (by simp;decide)) (K 2 (by simp; decide))
 #eval isSubGraph (K 3 (by simp;decide)) (K 4 (by simp; decide))
-#eval isSubGraph (K 3 (by simp;decide)) (Graph.mk ((K 3 (by simp;decide)).N.insert 4) (K 3 (by simp;decide)).E (by simp; decide))
 
 @[simp]
-def isomorphism (G H : Graph) (f_n : Node -> Node) (f_e : Edge -> Edge) : Prop :=
-  if (List.map f_n G.N) = H.N ∧ (List.map f_e G.E) = H.E then true else false
+def Isomorphism (G H : Graph) (f_n : Node -> Node) (f_e : Edge -> Edge) : Prop :=
+  (List.map f_n G.N) = H.N ∧ (List.map f_e G.E) = H.E
 
-@[simp]
-instance : Decidable (isomorphism G H f_n f_e) := by
-  rw [isomorphism]
-  simp
+instance : Decidable (Isomorphism G H f_n f_e) := by
+  rw [Isomorphism]
+
   exact instDecidableAnd
 
 #eval List.map (Nat.add 1 ·) (K 3 (by simp;decide)).N
 #eval List.map (fun x => Edge.mk x.id (x.i + 1) (x.j + 1)) (K 3 (by simp;decide)).E
 def H := Graph.mk (List.map (Nat.add 1 ·) (K 3 (by simp;decide)).N) (List.map (fun x => Edge.mk x.id (x.i + 1) (x.j + 1)) (K 3 (by simp;decide)).E) (by simp; decide)
-#eval isomorphism (K 3 (by simp;decide)) H (Nat.add 1 ·) (fun x => Edge.mk x.id (x.i + 1) (x.j + 1))
+#eval Isomorphism (K 3 (by simp;decide)) H (Nat.add 1 ·) (fun x => Edge.mk x.id (x.i + 1) (x.j + 1))
 
 def K5 : Graph := K 5 (by simp;decide)
 def K33 : Graph := Graph.mk [1,2,3,4,5,6] [(Edge.mk 1 1 4), (Edge.mk 2 1 5), (Edge.mk 3 1 6),(Edge.mk 4 2 4), (Edge.mk 5 2 5), (Edge.mk 6 2 6),(Edge.mk 7 3 4), (Edge.mk 8 3 5), (Edge.mk 9 3 6)] (by simp)
 
+-- the instances below were defined when trying to prove the decidability of planarity
 
-@[simp]
-instance : Decidable (isomorphism G K33 f_n f_e ∨ isomorphism G K5 f_n f_e) := by
-  exact instDecidableOr
+instance : Decidable (isSubGraph H G ∧ (Isomorphism H K33 f_n f_e ∨ Isomorphism H K5 f_n f_e)) := by
+  rw [Isomorphism]
+  rw [Isomorphism]
+  rw [isSubGraph]
+  exact instDecidableAnd
 
+def isSG (G H: Graph) :=  isSubGraph G H
+def isAdj (G : Graph) (f_n : Node -> Node) (f_e : Edge -> Edge):=  Isomorphism G K33 f_n f_e ∨ Isomorphism G K5 f_n f_e
 
-instance : Decidable (∃ H f_n f_e, isSubGraph H G ∧ isomorphism H K33 f_n f_e ∨ isomorphism H K5 f_n f_e) := by
-  unfold isomorphism
+instance : Decidable (isSG G H) := by
+  rw [isSG]
+  exact instDecidableIsSubGraph
+
+instance : Decidable (∃ f_n f_e, Isomorphism G K33 f_n f_e ∨ Isomorphism G K5 f_n f_e) := by
   simp
+  unfold List.map
+  by_cases h : G.N = []
+  rw [h]
+  simp
+  have h : K33.N = [1,2,3,4,5,6] := by rfl
+  have h2 : K5.N = [1,2,3,4,5] := by rfl
+  have h3 : K5.N ≠ [] := by rw [h2]; simp
+  rw [h, h2]
+  simp
+  apply instDecidableFalse
+  have h1 : G.N ≠ [] := by apply h
   sorry
 
+instance : Decidable (isAdj G f_n f_e) := by
+  rw [isAdj]
+  simp
+  exact instDecidableOr
 
-def isPlanar (G : Graph) : Bool :=
-if (∃ H f_n f_e, isSubGraph H G ∧ (isomorphism H K33 f_n f_e) ∨ (isomorphism H K5 f_n f_e))
+-- two implementations of planarity that can't be used because of the absence of a proof of decidability
+
+structure Planarity where
+  H : Graph
+  isPlanar := ∃G f_n f_e, ¬(isAdj G f_n f_e) ∧ isSG G H -- not possible to prove decidability
+deriving Repr
+
+instance : Decidable (∃ H f_n f_e, isSubGraph H G ∧ (Isomorphism H K33 f_n f_e ∨ Isomorphism H K5 f_n f_e)) :=
+  by sorry
+
+def isPlanar (G : Graph) : Prop :=
+if (∃H f_n f_e, (isSubGraph H G ) ∧ (Isomorphism H K33 f_n f_e ∨ Isomorphism H K5 f_n f_e))
 then false else true
 
 instance : Decidable (isPlanar G) := by
   rw [isPlanar]
   exact
-    (if ∃ H f_n f_e, isSubGraph H G ∧ isomorphism H K33 f_n f_e ∨ isomorphism H K5 f_n f_e then
+    (if ∃ H f_n f_e, isSubGraph H G ∧ (Isomorphism H K33 f_n f_e ∨ Isomorphism H K5 f_n f_e) then
           false
         else true).decEq
       true
